core/properties/forward_traceability/Forward_Traceability_link.v
@@ -1,0 +1,80 @@
+Require Import String.
+Require Import EqNat.
+Require Import List.
+Require Import PeanoNat.
+Require Import Lia.
+Require Import FunctionalExtensionality.
+
+Require Import core.Semantics.
+Require Import core.Syntax.
+Require Import core.Model.
+Require Import core.TransformationConfiguration.
+Require        core.Certification.
+Require Import core.utils.Utils.
+
+Require Import core.modeling.ConcreteSyntax.
+Require Import core.modeling.ModelingSemantics.
+Require Import core.modeling.ModelingMetamodel.
+Require Import core.modeling.ConcreteExpressions.
+Require Import core.modeling.Parser.
+
+
+
+(*************************************************************)
+(** * Forward_Traceability of CoqTL (Link)                   *)
+(** * Using operational semantics                            *)
+(*************************************************************)
+
+(** intuitively: I do not miss source elements, a.k.a. 
+                 it does not exist a situation where a (transformed) source pattern is not connected to any target element*)
+
+Definition Forward_Traceability_links {tc: TransformationConfiguration} (tr: Transformation) :=
+forall (sm : SourceModel) (tl : TargetLinkType),
+    (exists (sp : InputPiece),
+        In sp (allTuples tr sm) /\
+        In tl (LegacySemantics.applyTrOnPiece tr sm sp)) -> 
+        In tl (execute tr sm).(modelLinks) .
+
+Theorem forall_Forward_Traceability_links {tc:TransformationConfiguration} :
+forall (tr: Transformation), Forward_Traceability_links tr.
+Proof.
+    unfold Forward_Traceability_links.
+    apply Certification.tr_execute_in_links_legacy.
+Qed.
+
+
+
+
+
+
+
+
+
+
+
+
+
+
+
+
+
+
+(*
+
+(** FIXME M.T. different ways to write Forward_Traceability *)
+(**            we want to choose the one that is duality of *)
+(**            Backward_Traceability.  *)
+
+Theorem Totality_link:
+forall (tr: Transformation) (sm : SourceModel) (sp : InputPiece) (tl : TargetLinkType),
+In sp (allTuples tr sm) -> 
+In tl (applyOnPiece tr sm sp) ->
+In tl (allModelLinks (execute tr sm)).
+Proof.
+    intros.
+    apply tr_execute_in_links.
+    eexists sp. 
+    auto.
+Qed.
+
+*)
